ironfleet/src/Dafny/Distributed/Protocol/FailureDetector/Proof.i.dfy
@@ -1,0 +1,12 @@
+include "DistributedSystem.dfy"
+
+
+module FailureDetector_Detector {
+import opened FailureDetector_DistributedSystem
+
+predicate Assumption(s:TFD_State)
+{
+
+}
+
+}
