ironfleet/src/Dafny/Distributed/Protocol/FailureDetector/TimestampedDistributedSystem.i.dfy
@@ -1,0 +1,39 @@
+include "DistributedSystem.dfy"
+include "Timestamps/TimestampedType.dfy"
+
+module FailureDetector_TimestampedDistributedSystem {
+import opened FDTimestampedEnv_s
+import opened FailureDetector_DistributedSystem
+
+
+type TimestampedAgent = TimestampedType<Agent>
+
+datatype TFD_State = TFD_State(
+  config:Config,
+  t_environment:TimestampedLEnvironment<EndPoint, FDMessage, FDStep>,
+  t_servers:map<EndPoint,TimestampedAgent>
+  )
+
+  function UntagFDState(s:TFD_State) : FD_State
+  {
+    FD_State(
+      UntagLEnvironment(s.t_environment),
+      (map id | id in s.t_servers :: s.t_servers[id].v)
+      )
+  }
+
+  predicate TFD_Init(config:Config, s:TFD_State, heartbeatInterval:int, timeoutInterval:int)
+  {
+    && FD_Init(config, UntagFDState(s), heartbeatInterval, timeoutInterval)
+      && s.config == config
+      && LEnvironment_Init(s.t_environment)
+      && forall id :: id in s.t_servers ==> s.t_servers[id].ts == TimeZero()
+  }
+
+  predicate TFD_NextOneServer(s:TFD_State, s':TFD_State, actor:EndPoint, ios:seq<TimestampedLIoOp<EndPoint, FDMessage>>, hstep:FDStep)
+  {
+    && actor in s.t_servers
+    && FD_NextOneServer(UntagFDState(s), UntagFDState(s'), actor, UntagLIoOpSeq(ios))
+      && s.t_environment.nextStep.nodeStep == hstep
+  }
+}
