ironfleet/src/Dafny/Distributed/Protocol/FailureDetector/Timestamps/TimestampedType.dfy
@@ -1,0 +1,82 @@
+include "../../../Common/Framework/Environment.s.dfy"
+include "Timestamp.dfy"
+
+module FDTimestampedEnv_s {
+  import opened Environment_s
+  import opened FDTimestamp_s
+  import opened Collections__Seqs_i
+
+  datatype TimestampedType<Type> = TimestampedType(v:Type, ts:Timestamp)
+
+  type TimestampedLPacket<IdType, MessageType(==)> = LPacket<IdType, TimestampedType<MessageType>>
+
+  type TimestampedLIoOp<IdType, MessageType(==)> = LIoOp<IdType, TimestampedType<MessageType>>
+
+  type TimestampedLEnvStep<IdType, MessageType(==), NodeStepType> = LEnvStep<IdType,TimestampedType<MessageType>, NodeStepType>
+
+  type TimestampedLHostInfo<IdType, MessageType(==)> = LHostInfo<IdType,TimestampedType<MessageType>>
+
+  type TimestampedLEnvironment<IdType, MessageType(==), NodeStepType> = LEnvironment<IdType, TimestampedType<MessageType>, NodeStepType>
+
+  function UntagTimestampedType<T>(t_t: TimestampedType<T>) : T
+  {
+    t_t.v
+  }
+
+  function UntagLPacket<I,M>(pkt: TimestampedLPacket<I,M>) : LPacket<I,M>
+  {
+    LPacket(pkt.dst, pkt.src, pkt.msg.v)
+  }
+
+  function UntagSentPkts<I,M>(t_sentPkts : set<TimestampedLPacket<I,M>>) : set<LPacket<I,M>>
+  {
+    set pkt | pkt in t_sentPkts :: UntagLPacket(pkt)
+  }
+
+  function UntagLEnvStep(t_nextStep : TimestampedLEnvStep) : LEnvStep
+  {
+    match t_nextStep
+    {
+      case LEnvStepHostIos(actor, ios, nodeStep) => LEnvStepHostIos(actor, UntagLIoOpSeq(ios), nodeStep)
+      case LEnvStepDeliverPacket(p) => LEnvStepDeliverPacket(UntagLPacket(p))
+      case LEnvStepAdvanceTime() => LEnvStepAdvanceTime
+      case LEnvStepStutter() => LEnvStepStutter
+    }
+  }
+
+  function UntagHostInfo(t_hi: TimestampedLHostInfo) : LHostInfo
+  {
+    LHostInfo(MapSeqToSeq(t_hi.queue, UntagLPacket))
+  }
+
+  function UntagHostInfoMap<I,M>(t_hostInfo:map<I, LHostInfo<I,TimestampedType<M>>>) : map<I,LHostInfo<I,M>>
+  {
+    map id | id in t_hostInfo :: UntagHostInfo(t_hostInfo[id])
+  }
+
+  function UntagLEnvironment<I,M,S>(t_env: TimestampedLEnvironment<I,M,S>) : LEnvironment<I,M,S>
+  {
+    LEnvironment(t_env.time,
+      UntagSentPkts(t_env.sentPackets),
+      UntagHostInfoMap(t_env.hostInfo),
+      UntagLEnvStep(t_env.nextStep))
+  }
+
+  function UntagLIoOp(t_io : TimestampedLIoOp) : LIoOp
+  {
+    match t_io
+    {
+      case LIoOpSend(s) => LIoOpSend(UntagLPacket(s))
+      case LIoOpReceive(r) => LIoOpReceive(UntagLPacket(r))
+      case LIoOpTimeoutReceive() => LIoOpTimeoutReceive()
+      case LIoOpReadClock(t) => LIoOpReadClock(t)
+    }
+  }
+
+  function {:opaque} UntagLIoOpSeq(t_ios: seq<TimestampedLIoOp>) : seq<LIoOp>
+    ensures |UntagLIoOpSeq(t_ios)| == |t_ios|
+    ensures forall i :: 0 <= i < |UntagLIoOpSeq(t_ios)| ==> UntagLIoOpSeq(t_ios)[i] == UntagLIoOp(t_ios[i])
+  {
+    MapSeqToSeq(t_ios, UntagLIoOp)
+  }
+}
